add caller's footprint to lts

common/CategoricalComp.v
@@ -1,26 +1,44 @@
 Require Import Relations.
 Require Import List.
 Require Import Coqlib.
-Require Import LanguageInterface_ Events Globalenvs SmallstepLinking Smallstep_.
+Require Import LanguageInterface.
+Require Import Events.
+Require Import Globalenvs.
+Require Import SmallstepLinking.
+Require Import Smallstep_.
+Require Import Integers.
+Require Import Linking.
+Require Import AST.
 
 Open Scope smallstep_scope.
 Delimit Scope smallstep_scope with smallstep.
 
 Section COMP.
-  Context {liA liB liC S1 S2} (L1: lts liB liC S1) (L2: lts liA liB S2).
+  Context {liA liB liC} (Lsem1: semantics liB liC) (Lsem2: semantics liA liB).
+  Context (se: Genv.symtbl) (qset: ident -> Prop).
+  Let L1 := Lsem1 se.
+  Let Li1 := Lsem1 se qset.
+  Let L2 := Lsem2 se.
+  Let Li2 := Lsem2 se (fun i => footprint L1 i \/ qset i).
 
-  Variant comp_state := | st1 (s: S1) | st2 (s1: S1) (s2: S2).
+  Definition valid_query' {li} (q: query li): Prop :=
+    exists i, qset i /\ Genv.symbol_address se i Ptrofs.zero = entry q.
+
+  Variant comp_state :=
+  | st1 (s: state Lsem1) | st2 (s1: state Lsem1) (s2: state Lsem2).
 
   Inductive comp_step: comp_state -> trace -> comp_state -> Prop :=
   | step1 s1 t s1':
-      Step L1 s1 t s1' ->
+      Step Li1 s1 t s1' ->
       comp_step (st1 s1) t (st1 s1')
   | step2 s1 s2 t s2':
-      Step L2 s2 t s2' ->
+      Step Li2 s2 t s2' ->
       comp_step (st2 s1 s2) t (st2 s1 s2')
   | step_push s1 q s2:
       at_external L1 s1 q ->
       initial_state L2 q s2 ->
+      not (valid_query L1 se q) ->
+      not (valid_query' q) ->
       comp_step (st1 s1) E0 (st2 s1 s2)
   | step_pop s1 r s2 s1':
       final_state L2 s2 r ->
@@ -30,11 +48,12 @@ Section COMP.
   Inductive comp_initial_state (q: query liC): comp_state -> Prop :=
   | comp_initial_state_intro s:
       initial_state L1 q s ->
-      (* and the there exists the next step for s *)
       comp_initial_state q (st1 s).
 
   Inductive comp_at_external: comp_state -> query liA -> Prop :=
   | comp_at_external_intro s1 s2 (q: query liA):
+      not (valid_query L1 se q) ->
+      not (valid_query L2 se q) ->
       at_external L2 s2 q ->
       comp_at_external (st2 s1 s2) q.
 
@@ -48,108 +67,108 @@ Section COMP.
       final_state L1 s r ->
       comp_final_state (st1 s) r.
 
-  Definition comp_lts :=
+  Definition comp_lts_internal :=
     {|
     step ge := comp_step;
-    valid_query q := valid_query L1 q || valid_query L2 q;
+    globalenv := tt;
+    |}.
+  Definition comp_lts_external :=
+    {|
+    footprint i := footprint L1 i \/ footprint L2 i;
     initial_state := comp_initial_state;
     at_external := comp_at_external;
     after_external := comp_after_external;
     final_state := comp_final_state;
-    globalenv := tt;
     |}.
-
-  (* Definition comp_semantics sk: semantics liA liC := *)
-  (*   {| *)
-  (*   activate se := *)
-  (*     {| *)
-  (*       step ge := comp_step se; *)
-  (*       valid_query q := valid_query (L1 se) q || valid_query (L2 se) q; *)
-  (*       initial_state := comp_initial_state se; *)
-  (*       at_external := comp_at_external se; *)
-  (*       after_external := comp_after_external se; *)
-  (*       final_state := comp_final_state se; *)
-  (*       globalenv := tt; *)
-  (*     |}; *)
-  (*   skel := sk; *)
-  (*   |}. *)
 End COMP.
 
-Section ID.
-  Context {li: language_interface}.
-  Variant id_state :=
-  | st_q (q: query li)
-  | st_r (r: reply li).
-
-  Inductive id_step: id_state -> trace -> id_state -> Prop := .
-
-  Inductive id_initial_state: query li -> id_state -> Prop :=
-  | id_initial_state_intro q:
-      id_initial_state q (st_q q).
-
-  Inductive id_at_external: id_state -> query li -> Prop :=
-  | id_at_external_intro q:
-      id_at_external (st_q q) q.
-
-  Inductive id_after_external: id_state -> reply li -> id_state -> Prop :=
-  | id_after_external_intro q r:
-      id_after_external (st_q q) r (st_r r).
-
-  Inductive id_final_state: id_state -> reply li -> Prop :=
-  | id_final_state_intro r:
-      id_final_state (st_r r) r.
-
-  Definition id_lts :=
+Definition comp_semantics' {liA liB liC} (L1: semantics liB liC)
+           (L2: semantics liA liB) sk: semantics liA liC :=
+  {|
+  activate se :=
     {|
-    step ge := id_step;
-    valid_query q := false;
-    initial_state := id_initial_state;
-    at_external := id_at_external;
-    after_external := id_after_external;
-    final_state := id_final_state;
-    globalenv := tt;
-    |}.
-  (* Definition id_semantics sk: semantics li li := *)
-  (*   {| *)
-  (*   activate se := *)
-  (*     {| *)
-  (*       step ge := id_step; *)
-  (*       valid_query q := false; *)
-  (*       initial_state := id_initial_state; *)
-  (*       at_external := id_at_external; *)
-  (*       after_external := id_after_external; *)
-  (*       final_state := id_final_state; *)
-  (*       globalenv := tt; *)
-  (*     |}; *)
-  (*   skel := sk; *)
-  (*   |}. *)
-End ID.
+      steps p := comp_lts_internal L1 L2 se p;
+      events := comp_lts_external L1 L2 se;
+    |};
+    skel := sk;
+  |}.
 
-Definition fsim_lts {liA liB S1 S2} (L1: lts liA liB S1) (L2: lts liA liB S2) :=
-  exists index order ms, forall se,fsim_properties 1 1 se se tt L1 L2 index order ms.
-Definition equiv_lts {liA liB S1 S2} (L1: lts liA liB S1) (L2: lts liA liB S2) :=
-  fsim_lts L1 L2 /\ fsim_lts L2 L1.
+Definition comp_semantics {liA liB liC} (L1: semantics liB liC)
+           (L2: semantics liA liB): option (semantics liA liC) :=
+  option_map (comp_semantics' L1 L2) (link (skel L1) (skel L2)).
 
-Lemma fsim_lts_trivial_order {liA liB S1 S2} (L1: lts liA liB S1) (L2: lts liA liB S2):
-  (exists ms, forall se, fsim_properties 1 1 se se tt L1 L2 S1 (ltof _ (fun _ => O)) ms) -> fsim_lts L1 L2.
-Proof.
-  intros H. exists S1, (ltof _ (fun _ => O)). apply H.
-Qed.
+(* Section ID. *)
+(*   Context {li: language_interface}. *)
+(*   Variant id_state := *)
+(*   | st_q (q: query li) *)
+(*   | st_r (r: reply li). *)
+
+(*   Inductive id_step: id_state -> trace -> id_state -> Prop := . *)
+
+(*   Inductive id_initial_state: query li -> id_state -> Prop := *)
+(*   | id_initial_state_intro q: *)
+(*       id_initial_state q (st_q q). *)
+
+(*   Inductive id_at_external: id_state -> query li -> Prop := *)
+(*   | id_at_external_intro q: *)
+(*       id_at_external (st_q q) q. *)
+
+(*   Inductive id_after_external: id_state -> reply li -> id_state -> Prop := *)
+(*   | id_after_external_intro q r: *)
+(*       id_after_external (st_q q) r (st_r r). *)
+
+(*   Inductive id_final_state: id_state -> reply li -> Prop := *)
+(*   | id_final_state_intro r: *)
+(*       id_final_state (st_r r) r. *)
+
+(*   Definition id_lts := *)
+(*     {| *)
+(*     step ge := id_step; *)
+(*     footprint q := False; *)
+(*     initial_state := id_initial_state; *)
+(*     at_external := id_at_external; *)
+(*     after_external := id_after_external; *)
+(*     final_state := id_final_state; *)
+(*     globalenv := tt; *)
+(*     |}. *)
+(* End ID. *)
+
+(* Definition id_semantics {li} sk: semantics li li := *)
+(*   {| *)
+(*   activate se qset := id_lts; *)
+(*   skel := sk; *)
+(*   |}. *)
+
+
+(* Definition fsim_lts {liA liB S1 S2} (L1: lts liA liB S1) (L2: lts liA liB S2) := *)
+(*   exists index order ms, forall se,fsim_properties 1 1 se se tt L1 L2 index order ms. *)
+(* Definition equiv_lts {liA liB S1 S2} (L1: lts liA liB S1) (L2: lts liA liB S2) := *)
+(*   fsim_lts L1 L2 /\ fsim_lts L2 L1. *)
+
+(* Lemma fsim_lts_trivial_order {liA liB S1 S2} (L1: lts liA liB S1) (L2: lts liA liB S2): *)
+(*   (exists ms, forall se, fsim_properties 1 1 se se tt L1 L2 S1 (ltof _ (fun _ => O)) ms) -> fsim_lts L1 L2. *)
+(* Proof. *)
+(*   intros H. exists S1, (ltof _ (fun _ => O)). apply H. *)
+(* Qed. *)
 
 (* Definition forward_simulation' {liA liB} (L1 L2: semantics liA liB) := *)
 (*   forward_simulation 1 1 L1 L2. *)
 (* Definition equiv_simulation {liA liB} (L1 L2: semantics liA liB) := *)
 (*   forward_simulation' L1 L2 /\ forward_simulation' L2 L1. *)
 
-Notation "L1 ≤ L2" :=  (fsim_lts L1 L2)(at level 90): lts_scope.
-Notation "L1 ≡ L2" :=  (equiv_lts L1 L2)(at level 90): lts_scope.
-Notation "L1 ∘ L2" :=  (comp_lts L1 L2)(at level 40, left associativity): lts_scope.
-Notation " 1 " :=  (id_lts): lts_scope.
+Notation "L1 ≤ L2" :=  (forward_simulation 1 1 L1 L2)(at level 70): lts_scope.
 Open Scope lts_scope.
 Delimit Scope lts_scope with lts.
 
+Definition equiv_simulation {liA liB} (L1 L2: semantics liA liB) :=
+  L1 ≤ L2 /\ L2 ≤ L1.
+
+Notation "L1 ≡ L2" :=  (equiv_simulation L1 L2)(at level 90): lts_scope.
+Notation "L1 ∘ L2" :=  (comp_semantics L1 L2)(at level 40, left associativity): lts_scope.
+(* Notation " 1 " :=  (id_semantics): lts_scope. *)
+
 Section IDENTITY.
-  Context {liA liB S} (L : lts liA liB S).
+  Context {liA liB} (L : semantics liA liB).
 
   (* src q --initial_state--> ι1(ι1(q)) --step-->ι2(ι1(q),s)
 
@@ -157,79 +176,131 @@ Section IDENTITY.
 
      There's no appropriate way to match the intermediate state in the source
      program with the target program states *)
-  Lemma identity1: 1 ∘ L ≤ L.
-  Admitted.
+  (* Lemma identity1: 1 ∘ L ≤ L. *)
+  (* Admitted. *)
 
   (* src s ------------------final_state---------------> r
 
      tgt ι2(ι1(s)) ---step--> ι1(ι2(r)) --final_state--> r
 
      Similar issue with `final_state` being too strict *)
-  Lemma identity2: L ≤ 1 ∘ L.
-  Admitted.
+  (* Lemma identity2: L ≤ 1 ∘ L. *)
+  (* Admitted. *)
 
-  Theorem categorical_comp_left_identity: 1 ∘ L ≡ L.
-  Admitted.
+  (* Theorem categorical_comp_left_identity: 1 ∘ L ≡ L. *)
+  (* Admitted. *)
   (* Dually, the right identity law suffers from the same problem with
      `at_external` and `after_external` being too strict *)
-  Theorem categorical_comp_right_identity: L ∘ 1 ≡ L.
-  Admitted.
+  (* Theorem categorical_comp_right_identity: L ∘ 1 ≡ L. *)
+  (* Admitted. *)
 
 End IDENTITY.
 
+Lemma qset_step {liA liB S} (L: lts liA liB S) p1 p2 s t s':
+  Step (L p1) s t s' -> p1 = p2 -> Step (L p2) s t s'.
+Proof.
+  now intros H [ ].
+Qed.
+
+Require Import Coq.Logic.ClassicalFacts.
+Require Import Coq.Logic.FunctionalExtensionality.
+Axiom EquivThenEqual: prop_extensionality.
+
 Section ASSOC.
 
-  Context {liA liB liC liD S1 S2 S3}
-          (L1: lts liC liD S1) (L2: lts liB liC S2) (L3: lts liA liB S3).
+  Context {liA liB liC liD} (L1: semantics liC liD)
+          (L2: semantics liB liC) (L3: semantics liA liB).
+  Context (sk1 sk2 sk: AST.program unit unit).
 
-  Inductive assoc_state_match:
-    @comp_state S1 (@comp_state S2 S3) -> @comp_state (@comp_state S1 S2) S3 -> Prop :=
-  | assoc_match1 s1: assoc_state_match (st1 s1) (st1 (st1 s1))
-  | assoc_match2 s1 s2: assoc_state_match (st2 s1 (st1 s2)) (st1 (st2 s1 s2))
-  | assoc_match3 s1 s2 s3: assoc_state_match (st2 s1 (st2 s2 s3)) (st2 (st2 s1 s2) s3).
+  Let L12 := comp_semantics' L1 L2 sk1.
+  Let L23 := comp_semantics' L2 L3 sk2.
+  Let L := comp_semantics' L12 L3 sk.
+  Let L' := comp_semantics' L1 L23 sk.
 
-  Lemma assoc1: L1 ∘ (L2 ∘ L3) ≤ L1 ∘ L2 ∘ L3.
+  Arguments st1 {_ _ _}.
+  Arguments st2 {_ _ _}.
+
+  Inductive assoc_state_match: comp_state L1 L23 -> comp_state L12 L3 -> Prop :=
+  | assoc_match1 s1: assoc_state_match
+                       (st1 L1 L23 s1)
+                       (st1 L12 L3 (st1 L1 L2 s1))
+  | assoc_match2 s1 s2: assoc_state_match
+                          (st2 L1 L23 s1 (st1 L2 L3 s2))
+                          (st1 L12 L3 (st2 L1 L2 s1 s2))
+  | assoc_match3 s1 s2 s3: assoc_state_match
+                             (st2 L1 L23 s1 (st2 L2 L3 s2 s3))
+                             (st2 L12 L3 (st2 L1 L2 s1 s2) s3).
+
+  (* Lemma assoc1: L1 ∘ (L2 ∘ L3) ≤ L1 ∘ L2 ∘ L3. *)
+  Lemma assoc1: L' ≤ L.
   Proof.
-    apply fsim_lts_trivial_order.
-    eexists. intros se.
-    eapply forward_simulation_step with (match_states := assoc_state_match).
-    - intros. inv H. cbn. now rewrite orb_assoc.
+    constructor. econstructor. reflexivity.
+    intros se _ [ ] qset [ ] Hse.
+    instantiate (1 := fun _ _ _ => _). cbn beta.
+    apply forward_simulation_step
+      with (match_states := assoc_state_match); cbn.
+    - intros. now rewrite or_assoc.
     - intros q _ s1 [ ] H. inv H.
       eexists. split; try repeat constructor; auto.
     - intros s1 s2 r Hs H. inv H. inv Hs.
       eexists. split; try repeat constructor; auto.
-    - intros s1 s2 q Hs Hext. inv Hext. inv H. inv Hs.
+    - intros s1 s2 q Hs Hext. inv Hext. inv H1. inv Hs.
       eexists tt, _. repeat apply conj; try repeat constructor; auto.
-      intros r _ s1' [ ] Haft. inv Haft. inv H4.
+      intros [i [[Hi1 | Hi2] ?]];
+        [ apply H; eexists; split; eauto |
+          apply H2; eexists; split; eauto ].
+      intros r _ s1' [ ] Haft. inv Haft. inv H8.
       eexists. split; try repeat constructor; auto.
     - intros s1 t s1' Hstep s2 Hs.
       inv Hstep.
       + inv Hs. eexists; split; try repeat constructor; auto.
       + inv H; inv Hs; eexists; (split; [ | constructor ]).
         * apply step1. now apply step2.
-        * now apply step2.
-        * eapply step_push; try constructor; eauto.
+        * apply step2. eapply qset_step. eauto.
+          apply functional_extensionality. intros x.
+          apply EquivThenEqual.
+          cbn. rewrite <- or_assoc. apply or_iff_compat_r.
+          apply or_comm.
+        * (* eapply step_push; try constructor; eauto. *)
+          eapply step_push; eauto.
+          constructor; auto.
+          -- intros [x [? ?]]. apply H3. eexists; split; eauto.
+          -- intros [x [[? | ?] ?]].
+             apply H3. eexists; split; eauto.
+             apply H2. eexists; split; eauto.
+          -- intros [x [? ?]]. apply H3. eexists; split; eauto.
         * eapply step_pop; try constructor; eauto.
       + inv H0. eexists; split; [ | constructor ].
         inv Hs. constructor. eapply step_push; eauto.
       + inv H. eexists; split; [ | constructor].
         inv Hs. constructor. econstructor; eauto.
+    - apply well_founded_ltof.
   Qed.
 
-  Lemma assoc2: L1 ∘ L2 ∘ L3 ≤ L1 ∘ (L2 ∘ L3).
+  (* Lemma assoc2: L1 ∘ L2 ∘ L3 ≤ L1 ∘ (L2 ∘ L3). *)
+  Lemma assoc2: L ≤ L'.
   Proof.
-    apply fsim_lts_trivial_order.
-    eexists. intros se.
-    eapply forward_simulation_step with (match_states := fun s1 s2 => assoc_state_match s2 s1).
-    - intros. inv H. cbn. now rewrite <- orb_assoc.
+    constructor. econstructor. reflexivity.
+    intros se _ [ ] qset [ ] Hse.
+    instantiate (1 := fun _ _ _ => _). cbn beta.
+    apply forward_simulation_step
+      with (match_states := fun s1 s2 => assoc_state_match s2 s1); cbn.
+    - intros i. now rewrite or_assoc.
     - intros q _ s1 [ ] H. inv H. inv H0.
       eexists; split; constructor; auto.
     - intros s1 s2 r Hs H. inv H. inv H0. inv Hs.
       eexists; split; constructor; auto.
     - intros s1 s2 q Hs Hext. inv Hext. inv Hs.
       eexists tt, _. repeat apply conj; try repeat constructor; auto.
-      intros r _ s1' [ ] Haft. inv Haft.
-      eexists; split; repeat constructor; auto.
+      + intros [x [? ?]]. apply H. eexists; split; eauto.
+        left; auto.
+      + intros [x [[|]]].
+        apply H. eexists; split; eauto. right. auto.
+        apply H0. eexists; split; eauto.
+      + intros [x [? ?]].  apply H. eexists; split; eauto.
+        right; auto.
+      + intros r _ s1' [ ] Haft. inv Haft.
+        eexists; split; repeat constructor; auto.
     - intros s1 t s1' Hstep s2 Hs.
       inv Hstep.
       + inv H; inv Hs; eexists; (split; [ | constructor ]).
@@ -238,17 +309,78 @@ Section ASSOC.
         * eapply step_push; try constructor; eauto.
         * eapply step_pop; try constructor; eauto.
       + inv Hs. eexists; split; repeat constructor; auto.
+        eapply qset_step. eauto.
+        apply functional_extensionality. intros x.
+        apply EquivThenEqual.
+        cbn. rewrite <- or_assoc. apply or_iff_compat_r.
+        apply or_comm.
       + inv H. inv Hs. eexists; split; constructor.
         eapply step_push; eauto.
+        intros [x [[|]]].
+        apply H3. eexists; split; eauto.
+        apply H2. eexists; split; eauto.
       + inv H0. inv Hs. eexists; split; constructor.
         eapply step_pop; eauto.
+    - apply well_founded_ltof.
   Qed.
 
-  Theorem categorical_comp_assoc: L1 ∘ (L2 ∘ L3) ≡ L1 ∘ L2 ∘ L3.
+  (* Theorem categorical_comp_assoc: L1 ∘ (L2 ∘ L3) ≡ L1 ∘ L2 ∘ L3. *)
+  Theorem categorical_comp_assoc: L' ≡ L.
   Proof.
     split; [ exact assoc1 | exact assoc2 ].
   Qed.
 End ASSOC.
+
+Section FSIM.
+  Context {liA1 liA2 liB1 liB2 liC1 liC2}
+          (cc1: callconv liA1 liA2)
+          (cc2: callconv liB1 liB2)
+          (cc3: callconv liC1 liC2)
+          (L1: semantics liB1 liC1) (L2: semantics liA1 liB1)
+          (L1': semantics liB2 liC2) (L2': semantics liA2 liB2).
+  Context (HL1: fsim_components cc2 cc3 L1 L1')
+          (HL2: fsim_components cc1 cc2 L2 L2')
+          (se1 se2: Genv.symtbl) (w : ccworld cc3) (qset: ident -> Prop)
+          (Hse: match_senv cc3 w se1 se2)
+          (Hse1: Genv.valid_for (skel L1) se1)
+          (Hse2: Genv.valid_for (skel L1') se1).
+
+  Variant index := | index1: fsim_index HL1 -> index
+  | index2: fsim_index HL1 -> fsim_index HL2 -> index.
+
+  Variant order: index -> index -> Prop :=
+  | order1 i1 i1': fsim_order HL1 i1 i1' ->
+      order (index1 i1) (index1 i1')
+  | order2 i1 i1' i2 i2': fsim_order HL2 i2 i2' ->
+      order (index2 i1 i2) (index2 i1' i2').
+
+  Inductive match_states: index -> comp_state L1 L2 -> comp_state L1' L2' -> Prop :=
+  | match_st1 i1 s1 s1':
+      fsim_match_states HL1 se1 se2 w i1 s1 s1' ->
+      match_states (index1 i1) (st1 L1 L2 s1) (st1 L1' L2' s1')
+  | match_st2 i1 i2 s1 s1' s2 s2' w':
+      fsim_match_states HL1 se1 se2 w i1 s1 s1' ->
+      fsim_match_states HL2 se1 se2 w' i2 s2 s2' ->
+      match_states (index2 i1 i2) (st2 L1 L2 s1 s2) (st2 L1' L2' s1' s2').
+
+  Lemma comp_semantics_simulation sk sk':
+    fsim_properties cc1 cc3 se1 se2 w qset
+                    (comp_semantics' L1 L2 sk se1)
+                    (comp_semantics' L1' L2' sk' se2)
+                    index order match_states.
+  Proof.
+    split; cbn.
+  Admitted.
+
+End FSIM.
+
+Section APPROX.
+  Context {liA liB liC} (L1: semantics liB liC) (L2: semantics liA liB).
+  Context (sk: AST.program unit unit).
+
+
+
+End APPROX.
 
 Section CALL_CONV_REF.
 
@@ -266,7 +398,7 @@ Section CALL_CONV_REF.
   Lemma ccref_to_fsim:
     exists index order ms,
     forall w se1 se2, match_senv cc w se1 se2 ->
-    Smallstep_.fsim_properties cc' cc se1 se2 w 1 1 index order (ms w se1 se2).
+                 Smallstep_.fsim_properties cc' cc se1 se2 w 1 1 index order (ms w se1 se2).
   Proof.
     exists unit%type. exists (ltof _ (fun _ => O)).
     exists (fun w _ _ _ => cc_state_match w).
